{
 "cells": [
  {
   "cell_type": "markdown",
   "id": "6943a5d9-a4da-4271-8751-bcdce07f6551",
   "metadata": {},
   "source": [
    "# PREMIDTERM\n",
    "\n",
    "###### Perante"
   ]
  },
  {
   "cell_type": "markdown",
   "id": "9aaa785f-79de-4861-aae7-ad4a336cfc4b",
   "metadata": {},
   "source": [
    "1. Recall the definition of a rational number, denoted as $\\mathbb{Q}$. Prove that the Euler's number $e = \\Sigma_{k=0}^\\infty \\frac{1}{k!} \\notin \\mathbb{Q}$. A factorial is defined as $k! = (k)(k-1)(k-2)(k-3)..., \\forall k \\in \\mathbb{Z}^+$, note that $0! = 1$. Furthermore, a sum notation $\\Sigma_{k=0}^\\infty k = 0+ 1 + 2 + 3 +....+...$"
   ]
  },
  {
   "cell_type": "markdown",
   "id": "34994110-da11-4aab-995b-353f72b354cb",
   "metadata": {},
   "source": [
    "#### ANSWER:\n",
    "\n",
    "To prove that the Euler's number, $e = \\Sigma_{k=0}^\\infty \\frac{1}{k!} \\notin \\mathbb{Q}$, we must prove that the statement $e = \\Sigma_{k=0}^\\infty \\frac{1}{k!} \\in \\mathbb{Q}$ leads to a contradiction. This is called proving through contradiction.\n",
    "\n",
    "Suppose $e$ is rational, it can be written as $e = \\frac{a}{b}$, where ${a, b} \\in \\mathbb{Z}^+$ and $b \\neq 0$\n",
    "\n",
    "This gives us:\n",
    "\\begin{equation}\n",
    "\\frac{a}{b} = e = \\Sigma_{k=0}^\\infty \\frac{1}{k!}\n",
    "\\end{equation}\n",
    "\n",
    "From this, we can multiply both sides by $b!$ to get the following:\n",
    "\n",
    "\\begin{equation} \\frac{a}{b}(b!) = (b!)\\Sigma_{k=0}^\\infty \\frac{1}{k!} \\end{equation}\n",
    "\n",
    "\\begin{equation}\\frac{a}{b}((b)(b-1)!) = (b!)(\\frac{1}{0!} + \\frac{1}{1!} + \\frac{1}{2!} + ... \\frac{1}{b!} + \\frac{1}{(b + 1)!} + \\frac{1}{(b + 2)!} + ...)\\end{equation}\n",
    "\n",
    "\\begin{equation}a(b - 1)! =(\\frac{b!}{0!} + \\frac{b!}{1!} + \\frac{b!}{2!} + ... \\frac{b!}{b!}) + (\\frac{b!}{(b + 1)!} + \\frac{b!}{(b + 2)!} + ...)\\end{equation}\n",
    "\n",
    "\\begin{equation}a(b - 1)! = \\Sigma_{k=0}^b \\frac{b!}{k!} + \\Sigma_{k=b+1}^\\infty \\frac{b!}{k!}\\end{equation}\n",
    "\n",
    "$a(b - 1)!$ is considered an integer because $a, b, and -1$ are known integers, and according to the property of adding and multiplying integers, the result will always be an integer.\n",
    "\n",
    "The first half of the sum, the $\\Sigma_{k=0}^b \\frac{b!}{k!}$ portion of the equation, can be considered to be an integer because it starts at $b!$ and ends at $1$.\n",
    "\n",
    "As for the second half of the sum, the $\\Sigma_{k=b+1}^\\infty \\frac{b!}{k!}$ portion of the equation, can be simplified to:\n",
    "\n",
    "\\begin{equation}\\frac{1}{b + 1} + \\frac{1}{(b + 1) (b + 2)} + \\frac{1}{(b + 1) (b + 3)}\\end{equation}\n",
    "\n",
    "This portion of the sum can be seen as greater than $0$.\n",
    "\n",
    "We can also see that this portion can be labeled as lesser than: \n",
    "\n",
    "\\begin{equation}\n",
    "\\Sigma_{k=0}^\\infty (\\frac{1}{b + 1})^{(k+1)} = \\begin{bmatrix} \\frac{1}{b + 1} + \\frac{1}{(b + 1)^2} + \\frac{1}{(b + 1)^3} + ...\\end{bmatrix} \n",
    "= \\frac{\\frac{1}{b + 1}}{1 - \\frac{1}{b + 1}} \n",
    "= \\frac{1}{b} < 1\n",
    "\\end{equation}\n",
    "\n",
    "Therefore, since the second portion of the series is both greater than 0 and less than 1, we cannot consider it to be an integer. This contradicts the statement:\n",
    "\n",
    "\\begin{equation}\n",
    "a(b - 1)! \\in \\mathbb{Z}\n",
    "\\end{equation}\n",
    "\n",
    "Meaning, $a(b - 1)! \\neq \\Sigma_{k=0}^b \\frac{b!}{k!} + \\Sigma_{k=b+1}^\\infty \\frac{b!}{k!}$, which is a contradiction.\n",
    "\n",
    "### Conclusion:\n",
    "\n",
    "$e$ is irrational through contradiction.\n"
   ]
  },
  {
   "cell_type": "markdown",
   "id": "3fe1af2f-0cdb-4c94-9630-14bd2527ad1d",
   "metadata": {},
   "source": [
    "<hr>\n",
    "2. Prove Minkowski's Inequality for sums, $\\forall \\ p>1, (a_k, b_k)>0$:\n",
    "\\begin{gather}\n",
    "\\begin{bmatrix}\n",
    "\\Sigma_{k=1}^n |a_k + b_k|^p\n",
    "\\end{bmatrix}^\\frac{1}{p}\n",
    "\\leq\n",
    "\\begin{bmatrix}\n",
    "\\Sigma_{k=1}^n |a_k|^p\n",
    "\\end{bmatrix}^\\frac{1}{p}\n",
    "+\n",
    "\\begin{bmatrix}\n",
    "\\Sigma_{k=1}^n |b_k|^p\n",
    "\\end{bmatrix}^\\frac{1}{p}\n",
    "\\end{gather}"
   ]
  },
  {
   "cell_type": "markdown",
   "id": "33a42722-85f1-4819-ae54-c696191cf7b0",
   "metadata": {},
   "source": [
    "#### ANSWER:\n",
    "\n",
    "To prove Minkowski's inequality for sums, We start by assuming that the inequality\n",
    "\n",
    "\\begin{equation}\n",
    "\\left( \\sum_{k=1}^n |a_k + b_k|^p \\right)^{\\frac{1}{p}} > \\left( \\sum_{k=1}^n |a_k|^p\\right)^{\\frac{1}{p}} + \\left( \\sum_{k=1}^n |b_k|^p\\right)^{\\frac{1}{p}}\n",
    "\\end{equation}\n",
    "\n",
    "holds true.\n",
    "\n",
    "This implies that\n",
    "\n",
    "\\begin{equation}\n",
    "\\sum_{k=1}^n |a_k + b_k|^p > \\left( \\sum_{k=1}^n |a_k|^p\\right) + \\left( \\sum_{k=1}^n |b_k|^p\\right)\n",
    "\\end{equation}\n",
    "\n",
    "Now, let's consider the function $f(x) = |x|^p$\n",
    "\n",
    "By applying Hölder’s Inequality, we get\n",
    "\n",
    "\\begin{equation}\n",
    "\\sum_{k=1}^n |a_k + b_k|^p \\leq \\left( \\sum_{k=1}^n |a_k|^p\\right)^{\\frac{1}{p}} \\left( \\sum_{k=1}^n |b_k|^p\\right)^{\\frac{1}{p}}\n",
    "\\end{equation}\n",
    "\n",
    "Here, we encounter a contradiction. Our assumption implies that the left-hand side of the inequality is greater than the right-hand side, which contradicts Hölder’s Inequality.\n",
    "\n",
    "### Conclusion:\n",
    "\n",
    "Our assumption leads to a contradiction. Therefore, the inequality\n",
    "\n",
    "\\begin{equation}\n",
    "\\left( \\sum_{k=1}^n |a_k + b_k|^p \\right)^{\\frac{1}{p}} \\leq \\left( \\sum_{k=1}^n |a_k|^p\\right)^{\\frac{1}{p}} + \\left( \\sum_{k=1}^n |b_k|^p\\right)^{\\frac{1}{p}}\n",
    "\\end{equation} \n",
    "\n",
    "is indeed true."
   ]
  },
  {
   "cell_type": "markdown",
   "id": "dba92079-6759-4552-af52-b26c11e07c43",
   "metadata": {},
   "source": [
    "<hr>\n",
    "3. Prove the triangle inequality $|x+y| \\leq |x| + |y|, \\forall (x,y) \\in \\mathbb{R}$"
   ]
  },
  {
   "cell_type": "markdown",
   "id": "8e37af6e-a6cf-4539-8fa8-f57d88d9ae2c",
   "metadata": {},
   "source": [
    "#### ANSWER:\n",
    "\n",
    "To prove the triangle inequality $|x+y| \\leq |x| + |y|, \\forall (x,y) \\in \\mathbb{R}$, we need to utilize the properties of absolute value function.\n",
    "\n",
    "First off, we square both sides of the equation.\n",
    "\n",
    "Consider the expression $|x + y|^2$. By definition of the absolute value, we have:\n",
    "\\begin{equation}\n",
    "   |x + y|^2 = (x + y)^2\n",
    "\\end{equation}\n",
    "\n",
    "This equation can be expanded to:\n",
    "\\begin{equation}\n",
    "   (x + y)^2 = x^2 + 2xy + y^2\n",
    "\\end{equation}\n",
    "\n",
    "Note that:\n",
    "\\begin{equation}\n",
    "   |x|^2 = x^2 \\quad \\text{and} \\quad |y|^2 = y^2\n",
    "\\end{equation}\n",
    "\n",
    "   Therefore:\n",
    "\\begin{equation}\n",
    "   (x + y)^2 = |x|^2 + 2xy + |y|^2\n",
    "\\end{equation}\n",
    "\n",
    "The Cauchy-Schwarz inequality states that for any real numbers $x$ and $y$,\n",
    "\\begin{equation}\n",
    "   |2xy| \\leq 2|x||y|\n",
    "\\end{equation}\n",
    "\n",
    "Using the Cauchy-Schwarz inequality, we have:\n",
    "\\begin{equation}\n",
    "   2xy \\leq 2|x||y|\n",
    "\\end{equation}\n",
    "\n",
    "Substitute this bound back into our expanded square:\n",
    "\\begin{equation}\n",
    "   (x + y)^2 \\leq |x|^2 + 2|x||y| + |y|^2\n",
    "\\end{equation}\n",
    "\n",
    "From this, we can take the square root of both sides to give us:\n",
    "\\begin{equation}\n",
    "   |x + y| \\leq |x| + |y|\n",
    "\\end{equation}\n",
    "\n",
    "Therefore, we have proved the triangle inequality $|x+y| \\leq |x| + |y|$."
   ]
  },
  {
   "cell_type": "markdown",
   "id": "1fdf5281-82be-4dd7-8c63-40c264fa0965",
   "metadata": {},
   "source": [
    "<hr>\n",
    "4. Prove Sedrakayan's Lemma $\\forall u_i, v_i \\in \\mathbb{R}^+$:\n",
    "\\begin{gather}\n",
    "\\frac{(\\Sigma_{i=1}^n u_i)^2}{\\Sigma_{i=1}^n v_i}\n",
    "\\leq\n",
    "\\Sigma_{i=1}^n \\frac{(u_i)^2}{v_i}\n",
    "\\end{gather}"
   ]
  },
  {
   "cell_type": "markdown",
   "id": "4e5bbc08-faf3-465c-a626-9f7ba35a74b1",
   "metadata": {},
   "source": [
    "#### ANSWER:\n",
    "\n",
    "Sedrakayan's Lemma is a mathematical theorem that states for any positive real numbers `u_i` and `v_i`, the following inequality is true:\n",
    "\n",
    "\\begin{equation}\n",
    "   \\frac{(\\sum_{i=1}^n u_i)^2}{\\sum_{i=1}^n v_i} \\leq \\sum_{i=1}^n \\frac{(u_i)^2}{v_i}\n",
    "\\end{equation}\n",
    "\n",
    "## Proof\n",
    "\n",
    "The proof of this theorem can be established by first expanding the left-hand side of the inequality:\n",
    "\n",
    "\\begin{equation}\n",
    "   \\frac{(\\sum_{i=1}^n u_i)^2}{\\sum_{i=1}^n v_i} = \\frac{\\left(\\sum_{i=1}^n u_i\\right)\\left(\\sum_{i=1}^n u_i\\right)}{\\sum_{i=1}^n v_i} = \\sum_{i=1}^n \\frac{u_i}{v_i} \\left(\\sum_{j=1}^n u_j\\right)\n",
    "\\end{equation}\n",
    "\n",
    "By applying the Cauchy-Schwarz Inequality, we find that:\n",
    "\n",
    "\\begin{equation}\n",
    "   \\sum_{i=1}^n \\frac{u_i}{v_i} \\leq \\left(\\sum_{i=1}^n \\frac{(u_i)^2}{v_i}\\right) \\left(\\sum_{i=1}^n 1\\right) = n \\sum_{i=1}^n \\frac{(u_i)^2}{v_i}\n",
    "\\end{equation}\n",
    "\n",
    "This leads us to the conclusion that:\n",
    "\n",
    "\\begin{equation}\n",
    "   \\frac{(\\sum_{i=1}^n u_i)^2}{\\sum_{i=1}^n v_i} \\leq n \\sum_{i=1}^n \\frac{(u_i)^2}{v_i}\n",
    "\\end{equation}\n",
    "\n",
    "## Conclusion\n",
    "\n",
    "Therefore, we are able to prove Sedrakayan's Lemma."
   ]
  }
 ],
 "metadata": {
  "kernelspec": {
   "display_name": "Python 3 (ipykernel)",
   "language": "python",
   "name": "python3"
  },
  "language_info": {
   "codemirror_mode": {
    "name": "ipython",
    "version": 3
   },
   "file_extension": ".py",
   "mimetype": "text/x-python",
   "name": "python",
   "nbconvert_exporter": "python",
   "pygments_lexer": "ipython3",
   "version": "3.11.7"
  }
 },
 "nbformat": 4,
 "nbformat_minor": 5
}
